new/proof/go_etcd_io/etcd/pkg/v3/wait.v
@@ -2,7 +2,7 @@ Require Export New.generatedproof.go_etcd_io.etcd.pkg.v3.wait.
 Require Export New.proof.proof_prelude.
 From New.proof Require Import log sync.
 From New.proof.github_com.goose_lang.goose.model.channel
-  Require Import logatom.chan_au_base idiom.handoff.handoff.
+  Require Import logatom.chan_au_base idiom.bag.bag.
 
 Section wps.
 Context `{hG: heapGS Σ, !ffi_semantics _ _}.
